src/tls/HMAC.UFCMA.fst
@@ -1,6 +1,4 @@
-(**
-Idealizing HMAC for Finished message payloads and binders.
-*)
+(**! Idealizing HMAC for Finished message payloads and Binders. *)
 module HMAC.UFCMA
 
 open FStar.Heap
@@ -21,8 +19,146 @@ open TLSError
 // for concreteness; the rest of the module is parametric in a:alg
 
 #set-options "--initial_fuel 1 --max_fuel 1 --initial_ifuel 1 --max_ifuel 1"
+//open IK 
+
 
 type rgn = TLSConstants.rgn
+type fresh_subregion rg parent h0 h1 = stronger_fresh_region rg h0 h1 /\ extends rg parent
+
+type ha = Hashing.Spec.alg 
+type text = bytes
+
+
+noeq type info: Type0 = { 
+  parent:rgn; 
+  alg:ha; 
+  good: text -> bool (*TODO: should be Type0 *)}
+
+type tag (u:info) = lbytes (Hashing.Spec.tagLen u.alg)
+
+let keylen (u:info): IK.keylen = UInt32.uint_to_t (Hashing.Spec.tagLen u.alg)
+type keyrepr (u:info) = lbytes (UInt32.v (keylen u))
+
+
+private type log_t
+  (#ip:IK.ipkg)
+  (i:ip.IK.t)
+  (u:info)
+  (r:rgn)
+= MonotoneMap.t r (tag u * text) (fun (t,v) -> _:unit{ip.IK.honest i ==> u.good v}) (fun _ -> True) // could constrain size
+
+// readers and writers share the same private state: a log of MACed messages
+noeq abstract type key (#ip:IK.ipkg) (i:ip.IK.t) (u:info) =
+  | Key:
+    #region: rgn{extends region u.parent} -> // intuitively, the writer's region
+    kv: keyrepr u ->
+    log: log_t i u region -> //TODO: make conditional
+    key i u
+
+val region: #ip:IK.ipkg -> #i:ip.IK.t -> #u:info -> key i u -> GTot rid
+val keyval: #ip:IK.ipkg -> #i:ip.IK.t -> #u:info -> key i u -> GTot (keyrepr u)
+
+let region #ip #i #u k  = k.region
+let keyval #ip #i #u k = k.kv
+
+private let gen (#ip:IK.ipkg) (i:ip.IK.t) (u:info) (kv:keyrepr u) : ST (key i u)
+  (requires (fun _ -> True))
+  (ensures (fun h0 k h1 ->
+    fresh_subregion (region k) u.parent h0 h1 /\
+    modifies Set.empty h0 h1
+  )) =
+  let region: r:rgn{extends r u.parent} = new_region u.parent in
+  let log: log_t #ip i u region = MonotoneMap.alloc #region #(tag u * text) #(fun (t,v) -> _:unit{ip.IK.honest i ==> u.good v}) #(fun _ -> True) in
+  Key kv log
+
+val create: #ip:IK.ipkg -> i:ip.IK.t -> u:info -> ST (key i u)
+  (requires (fun _ -> True))
+  (ensures (fun h0 k h1 ->
+    modifies Set.empty h0 h1 /\
+    fresh_subregion (region k) u.parent h0 h1 ))
+let create #ip i u =
+  gen i u (CoreCrypto.random (UInt32.v (keylen u)))
+
+val coerce: #ip:IK.ipkg -> i:ip.IK.t -> u:info -> kv:keyrepr u -> ST (key i u)
+  (requires (fun _ -> ~(ip.IK.honest i)))
+  (ensures (fun h0 k h1 ->
+    modifies Set.empty h0 h1 /\
+    fresh_subregion (region k) u.parent h0 h1 ))
+let coerce #ip i u kv = 
+  gen i u kv
+
+// not quite doable without reification?
+// assert_norm(forall ip i u. (create #ip i u == coerce #ip i u (CoreCrypto.random (UInt32.v (keylen u)))))
+
+val leak: #ip:IK.ipkg -> #i:ip.IK.t -> #u:info -> k:key i u {~(ip.IK.honest i)} -> kv:keyrepr u { kv = keyval k }
+let leak  #ip #i #u k = k.kv
+
+val mac: 
+  #ip:IK.ipkg -> #i:ip.IK.t -> #u:info -> k:key i u ->
+  p:text { ip.IK.honest i ==> u.good p } -> ST (tag u)
+  (requires (fun _ -> True))
+  (ensures (fun h0 t h1 -> modifies (Set.singleton (region k)) h0 h1
+  //  we may be more precise, e,g,  /\ sel h1 k.log = snoc (sel h0 k.log) (Entry t p)
+  ))
+
+
+let mac #ip #i #u k p =
+  //let p : p:bytes { ip.IK.honest i ==> u.good p } = p in
+  let t = HMAC.hmac u.alg k.kv p in
+  if None? (MonotoneMap.lookup k.log (t,p)) then MonotoneMap.extend k.log (t,p) ();
+  t
+
+//abstract val matches: #i:id -> #good:(bytes -> Type) -> p:text -> entry i good -> Tot bool
+//let matches #i #good p (Entry _ p') = p = p'
+
+val verify: 
+  #ip:IK.ipkg -> #i:ip.IK.t -> #u:info -> k:key i u ->
+  p:text -> t: tag u -> ST bool
+  (requires (fun _ -> True))
+  (ensures (fun h0 b h1 -> modifies Set.empty h0 h1 /\ (b /\ ip.IK.honest i ==> u.good p)))
+
+// We use the log to correct any verification errors
+let verify #ip #i #u k p t =
+  let verified = HMAC.hmacVerify u.alg k.kv p t in
+  let maced  = Some? (MonotoneMap.lookup k.log (t,p)) in
+  verified  &&
+  (not(ip.IK.honest i) || maced)
+
+
+let pkg (#ip:IK.ipkg) (u:info): IK.pkg ip = IK.Pkg
+  info
+  key
+  keylen
+  create
+  coerce
+
+/// Now entirely independent of TLS.
+/// 
+/// We'll use something of the form
+///
+/// let good text =
+///   exists digest.
+///     hashed ha digest /\
+///     text = hash ha digest /\ 
+///     witnessed (fun h -> "this is the writer's state is ...")
+///
+/// - how to deal with agility here?
+/// - which level of abstraction? 
+
+
+/// TODOs:
+/// - Type0/Type1
+/// - how to pass key-generation-time usage parameters?
+/// - how to guarantee matching goodnesses?
+/// - more specific instantiations? 
+/// (later) support dynamic key compromise
+
+
+
+
+/// ------------ older, TLS-specific implementation 
+
+//17-10-21 ADAPT: should depend only on agility parameter.
 
 type id =
 | HMAC_Finished of TLSInfo.finishedId
@@ -36,30 +172,14 @@ let alg (i:id) = match i with
 val authId: id -> Tot bool
 let authId id = false // TODO: move to Flags
 
-type text = bytes
-type tag (i:id) = lbytes (Hashing.Spec.tagLen (alg i))
+type tag (i:id) = tagr (alg i)
 
-let keysize (i:id) = Hashing.Spec.tagLen (alg i)
-type keyrepr (i:id) = lbytes (keysize i)
 
-type fresh_subregion rg parent h0 h1 = stronger_fresh_region rg h0 h1 /\ extends rg parent
-
+ 
 // We keep the tag in case we later want to enforce tag authentication
 abstract type entry (i:id) (good: bytes -> Type) =
   | Entry: t:tag i -> p:bytes { authId i ==> good p } -> entry i good
 
-// readers and writers share the same private state: a log of MACed messages
-// TODO make it abstract
-(*
- * AR: two changes: region is of type rgn.
- * log is a hyperstack ref with refinement capturing its rid.
- *)
-noeq type key (i:id) (good: bytes -> Type) =
-  | Key:
-    #region: rgn -> // intuitively, the writer's region
-    kv: keyrepr i ->
-    log: ref (seq (entry i good)){log.id = region} ->
-    key i good
 
 val region: #i:id -> #good:(bytes -> Type) -> k:key i good -> GTot rid
 val keyval: #i:id -> #good:(bytes -> Type) -> k:key i good -> GTot (keyrepr i)
@@ -92,7 +212,8 @@ val coerce: i:id -> good: (bytes -> Type) -> parent: rgn -> kv:keyrepr i -> ST(k
   (ensures (fun h0 k h1 ->
     modifies Set.empty h0 h1 /\
     fresh_subregion (region #i #good k) parent h0 h1 ))
-let coerce i good parent kv = gen0 i good parent kv
+let coerce i good parent kv = 
+  gen0 i good parent kv
 
 val leak: #i:id -> #good: (bytes -> Type) -> k:key i good {~(authId i)} -> Tot (kv:keyrepr i { kv = keyval k })
 let leak   #i #good k = k.kv
